systems/chord-props/RingCorrect.v
@@ -1,3 +1,5 @@
+Require Import List.
+
 Require Import Chord.Chord.
 Require Import Chord.SystemReachable.
 
@@ -22,3 +24,14 @@ Definition sufficient_principals (gst : global_state) : Prop :=
 Definition state_invariant (gst : global_state) : Prop :=
   sufficient_principals gst /\
   live_node_in_succ_lists gst.
+
+Lemma first_succ_and_others_distinct :
+  forall gst h st s1 s2 xs ys,
+    reachable_st gst ->
+    sigma gst h = Some st ->
+    succ_list st = xs ++ s1 :: ys ->
+    In s2 (xs ++ ys) ->
+    addr_of s1 <> addr_of s2.
+Proof.
+Admitted.
+Hint Resolve first_succ_and_others_distinct.
